CrGeneralProgramState.v
@@ -6,82 +6,138 @@ From MyProject Require Import SmtExpr.
 From Stdlib Require Import List.
 Import ListNotations.
 
-(* [Th] is the header-value type, [Tb] the packet-bit type. *)
-Record GeneralProgramState (Th Tb : Type) := {
+(* [Th] is the header-value type, [Tb] the packet-bit type, [Tm] the type of a
+   memory region's contents.
+
+   [Tm] is a third parameter rather than a reuse of [Th] because a region is
+   not a scalar: concretely it is an [Array CrVal], symbolically an
+   [SmtArrExpr].  Memory lives here rather than on [TransformerState] because
+   [TransformerState T] is homogeneous in a single element type -- see the
+   comment on [CrConcreteSemanticsTransformer.eval_transformer_concrete_mem]
+   for how it is threaded into a transformer instead.
+
+   [sh_mem_extent] is the memory analogue of [sh_bits_read]: per region, the
+   largest offset the run has touched.  Two programs that emit the same packet
+   while reaching different distances into a region are not interchangeable,
+   because one can fault where the other does not.  It is updated on every
+   access, in bounds or not, which is what lets loads and stores stay total. *)
+Record GeneralProgramState (Th Tb Tm : Type) := {
   sh_hdr_map : PMap.t Th;
   sh_read_tape : list Tb;
   sh_bits_read : Th;
   sh_write_tape : list Tb;
+  sh_mem : PMap.t Tm;
+  sh_mem_extent : PMap.t Th;
   mod_states : PMap.t (ModuleState Th Tb);
   gps_valid : Tb;
 }.
 
-Arguments sh_hdr_map {Th Tb} _.
-Arguments sh_read_tape {Th Tb} _.
-Arguments sh_bits_read {Th Tb} _.
-Arguments sh_write_tape {Th Tb} _.
-Arguments mod_states {Th Tb} _.
-Arguments gps_valid {Th Tb} _.
+Arguments sh_hdr_map {Th Tb Tm} _.
+Arguments sh_read_tape {Th Tb Tm} _.
+Arguments sh_bits_read {Th Tb Tm} _.
+Arguments sh_write_tape {Th Tb Tm} _.
+Arguments sh_mem {Th Tb Tm} _.
+Arguments sh_mem_extent {Th Tb Tm} _.
+Arguments mod_states {Th Tb Tm} _.
+Arguments gps_valid {Th Tb Tm} _.
 
-Definition set_gps_shared_headers {Th Tb : Type}
-  (gps : GeneralProgramState Th Tb) (hdrs : PMap.t Th)
-  : GeneralProgramState Th Tb :=
+Definition set_gps_shared_headers {Th Tb Tm : Type}
+  (gps : GeneralProgramState Th Tb Tm) (hdrs : PMap.t Th)
+  : GeneralProgramState Th Tb Tm :=
   {| sh_hdr_map := hdrs;
      sh_read_tape := sh_read_tape gps;
      sh_bits_read := sh_bits_read gps;
      sh_write_tape := sh_write_tape gps;
+     sh_mem := sh_mem gps;
+     sh_mem_extent := sh_mem_extent gps;
      mod_states := mod_states gps;
      gps_valid := gps_valid gps |}.
 
-Definition set_gps_shared_read_tape {Th Tb : Type}
-  (gps : GeneralProgramState Th Tb) (bits : list Tb)
-  : GeneralProgramState Th Tb :=
+Definition set_gps_shared_read_tape {Th Tb Tm : Type}
+  (gps : GeneralProgramState Th Tb Tm) (bits : list Tb)
+  : GeneralProgramState Th Tb Tm :=
   {| sh_hdr_map := sh_hdr_map gps;
      sh_read_tape := bits;
      sh_bits_read := sh_bits_read gps;
      sh_write_tape := sh_write_tape gps;
+     sh_mem := sh_mem gps;
+     sh_mem_extent := sh_mem_extent gps;
      mod_states := mod_states gps;
      gps_valid := gps_valid gps |}.
 
-Definition set_gps_bits_read {Th Tb : Type}
-  (gps : GeneralProgramState Th Tb) (n : Th)
-  : GeneralProgramState Th Tb :=
+Definition set_gps_bits_read {Th Tb Tm : Type}
+  (gps : GeneralProgramState Th Tb Tm) (n : Th)
+  : GeneralProgramState Th Tb Tm :=
   {| sh_hdr_map := sh_hdr_map gps;
      sh_read_tape := sh_read_tape gps;
      sh_bits_read := n;
      sh_write_tape := sh_write_tape gps;
+     sh_mem := sh_mem gps;
+     sh_mem_extent := sh_mem_extent gps;
      mod_states := mod_states gps;
      gps_valid := gps_valid gps |}.
 
-Definition set_gps_shared_write_tape {Th Tb : Type}
-  (gps : GeneralProgramState Th Tb) (cbits : list Tb)
-  : GeneralProgramState Th Tb :=
+Definition set_gps_shared_write_tape {Th Tb Tm : Type}
+  (gps : GeneralProgramState Th Tb Tm) (cbits : list Tb)
+  : GeneralProgramState Th Tb Tm :=
   {| sh_hdr_map := sh_hdr_map gps;
      sh_read_tape := sh_read_tape gps;
      sh_bits_read := sh_bits_read gps;
      sh_write_tape := cbits;
+     sh_mem := sh_mem gps;
+     sh_mem_extent := sh_mem_extent gps;
      mod_states := mod_states gps;
      gps_valid := gps_valid gps |}.
 
-Definition set_gps_mod_states {Th Tb : Type}
-  (gps : GeneralProgramState Th Tb) (ms : PMap.t (ModuleState Th Tb))
-  : GeneralProgramState Th Tb :=
+Definition set_gps_mem {Th Tb Tm : Type}
+  (gps : GeneralProgramState Th Tb Tm) (m : PMap.t Tm)
+  : GeneralProgramState Th Tb Tm :=
   {| sh_hdr_map := sh_hdr_map gps;
      sh_read_tape := sh_read_tape gps;
      sh_bits_read := sh_bits_read gps;
      sh_write_tape := sh_write_tape gps;
+     sh_mem := m;
+     sh_mem_extent := sh_mem_extent gps;
+     mod_states := mod_states gps;
+     gps_valid := gps_valid gps |}.
+
+Definition set_gps_mem_extent {Th Tb Tm : Type}
+  (gps : GeneralProgramState Th Tb Tm) (e : PMap.t Th)
+  : GeneralProgramState Th Tb Tm :=
+  {| sh_hdr_map := sh_hdr_map gps;
+     sh_read_tape := sh_read_tape gps;
+     sh_bits_read := sh_bits_read gps;
+     sh_write_tape := sh_write_tape gps;
+     sh_mem := sh_mem gps;
+     sh_mem_extent := e;
+     mod_states := mod_states gps;
+     gps_valid := gps_valid gps |}.
+
+Definition set_gps_mod_states {Th Tb Tm : Type}
+  (gps : GeneralProgramState Th Tb Tm) (ms : PMap.t (ModuleState Th Tb))
+  : GeneralProgramState Th Tb Tm :=
+  {| sh_hdr_map := sh_hdr_map gps;
+     sh_read_tape := sh_read_tape gps;
+     sh_bits_read := sh_bits_read gps;
+     sh_write_tape := sh_write_tape gps;
+     sh_mem := sh_mem gps;
+     sh_mem_extent := sh_mem_extent gps;
      mod_states := ms;
      gps_valid := gps_valid gps |}.
 
-Definition set_gps_valid {Th Tb : Type}
-  (gps : GeneralProgramState Th Tb) (valid : Tb)
-  : GeneralProgramState Th Tb :=
+Definition set_gps_valid {Th Tb Tm : Type}
+  (gps : GeneralProgramState Th Tb Tm) (valid : Tb)
+  : GeneralProgramState Th Tb Tm :=
   {| sh_hdr_map := sh_hdr_map gps;
      sh_read_tape := sh_read_tape gps;
      sh_bits_read := sh_bits_read gps;
      sh_write_tape := sh_write_tape gps;
+     sh_mem := sh_mem gps;
+     sh_mem_extent := sh_mem_extent gps;
      mod_states := mod_states gps;
      gps_valid := valid |}.
 
-Definition GeneralConcreteState : Type := GeneralProgramState CrVal bool.
-Definition GeneralSymbolicState : Type := GeneralProgramState SmtArithExpr (ConditionalVal SmtBoolExpr).
+Definition GeneralConcreteState : Type :=
+  GeneralProgramState CrVal bool (@Array CrVal).
+Definition GeneralSymbolicState : Type :=
+  GeneralProgramState SmtArithExpr (ConditionalVal SmtBoolExpr) SmtArrExpr.
